old/Impl.v
@@ -1,0 +1,83 @@
+Require Import
+  Coq.Arith.Arith
+  Coq.micromega.Lia
+  Lib
+  RSWE.
+
+From Equations Require Import Equations.
+Set Equations With UIP.
+
+Generalizable All Variables.
+
+Section Pact.
+
+Import ListNotations.
+
+Definition Gas : Type := nat.
+
+Variable r : Type.
+Variable s : Type.
+Variable w : Type.
+
+Inductive Err : Type :=
+  | Err_Raise.
+
+Definition PactM := @RSWE r s w Err.
+
+Definition app `(f : a → PactM b) (x : PactM a) : PactM b :=
+  gas <- getT ;
+  if 0 <? gas
+  then putT (gas - 1) ;;
+       x >>= f
+  else λ _, inl Err_CarNil.
+
+Equations compares {τ : Ty} (gas : Gas)
+          (p : PactM (PactTy τ)) (e : Err + SemTy τ) : Prop := {
+  compares gas p (inl err) with p gas := {
+    | inl err'       => err = err'
+    | inr x'         => False
+  };
+  compares gas p (inr x) with p gas := {
+    | inl err'       => False
+    | inr (x', gas') => compares_exp gas' (τ:=τ) x' x
+  }
+}
+where compares_exp {τ : Ty} (gas : Gas)
+                (p : PactTy τ) (e : SemTy τ) : Prop := {
+  compares_exp (τ:=TyUnit)     _   () () := True;
+  compares_exp (τ:=dom ⟶ cod) gas f' f  :=
+    ∀ (x' : PactTy dom) (x : SemTy dom),
+      compares_exp (τ:=dom) gas x' x → compares (τ:=cod) gas (f' x') (f x)
+}.
+
+Notation "x ~=[ gas ]=~ y" := (compares gas x y) (at level 100).
+
+Ltac simpler :=
+  repeat
+    (simpl;
+     simp compares; simpl;
+     unfold compares_clause_1; simpl;
+     unfold compares_clause_2; simpl;
+     unfold Prelude.apply; simpl).
+
+Ltac enough_gas gas :=
+  let H := fresh "H" in
+  destruct (lt_dec 0 gas) as [H|H];
+  [ apply Nat.ltb_lt in H;
+    rewrite H;
+    simpler
+  | try lia ].
+
+Lemma app_sound {dom cod : Ty}
+      (x : PactTy cod) (x' : SemTy cod) :
+  ∃ gas, ∀ gas', gas < gas' →
+    compares_exp (τ:=cod) (gas' - 1) x x' →
+    compares (τ:=cod) gas' (app pure (pure x)) (pure x').
+Proof.
+  unfold app.
+  exists 2; intros.
+  simpler.
+  now enough_gas gas'.
+Qed.
+
+End Pact.
