src/RWSE.v
@@ -1,0 +1,104 @@
+Require Import Hask.Prelude.
+Require Import Hask.Ltac.
+Require Import Hask.Control.Monad.
+Require Import Hask.Data.Monoid.
+Require Import Coq.Unicode.Utf8.
+
+Generalizable All Variables.
+Set Primitive Projections.
+Set Universe Polymorphism.
+Unset Transparent Obligations.
+
+(******************************************************************************
+ * The RWSET Monad transformer
+ *)
+
+Section RWSE.
+
+Context {r s w e : Type}.
+
+Definition RWSE (a : Type) := r → s → w → e + (a * (s * w)).
+
+Definition ask : RWSE r := λ r s w, inr (r, (s, w)).
+
+Definition local (f : r → r) `(x : RWSE a) : RWSE a :=
+  λ r s w, x (f r) s w.
+
+Definition get                : RWSE s    := λ r s w, inr (s, (s, w)).
+Definition gets `(f : s → a)  : RWSE a    := λ r s w, inr (f s, (s, w)).
+Definition put (x : s)        : RWSE unit := λ _ _ w, inr (tt, (x, w)).
+Definition modify (f : s → s) : RWSE unit := λ _ s w, inr (tt, (f s, w)).
+
+Definition tell `{Monoid w} (v : w) : RWSE unit :=
+  λ _ s w, inr (tt, (s, w ⨂ v)).
+
+Definition tellf (f : w → w) : RWSE unit := λ _ s w, inr (tt, (s, f w)).
+
+Definition throw (err : e) : RWSE unit := λ _ _ _, inl err.
+
+#[export]
+Program Instance RWSE_Functor : Functor RWSE := {
+  fmap := λ A B f (x : RWSE A), λ r s w, first f <$> x r s w
+}.
+
+Definition RWSE_ap {a b : Type} (f : RWSE (a → b)) (x : RWSE a) :
+  RWSE b := λ r s w,
+  match f r s w with
+  | inl e => inl e
+  | inr (f', (s', w')) => first f' <$> x r s' w'
+  end.
+
+#[export]
+Program Instance RWSE_Applicative : Applicative RWSE := {
+  pure := λ _ x, λ _ s w, inr (x, (s, w));
+  ap   := @RWSE_ap
+}.
+
+Definition RWSE_join `(x : RWSE (RWSE a)) :
+  RWSE a := λ r s w,
+  match x r s w with
+  | inl e => inl e
+  | inr (y, (s', w')) => y r s w
+  end.
+
+#[export]
+Program Instance RWSE_Monad : Monad RWSE := {
+  join := @RWSE_join
+}.
+
+End RWSE.
+
+Arguments RWSE r s w e a.
+
+Module RWSELaws.
+
+Require Import FunctionalExtensionality.
+
+Include MonadLaws.
+
+Lemma first_id : forall a z, first (a:=a) (b:=a) (z:=z) id = id.
+Proof.
+  unfold first.
+  intros a z.
+  extensionality x.
+  destruct x; auto.
+Qed.
+
+Program Instance RWSE_FunctorLaws {r s w e : Type} :
+  FunctorLaws (@RWSE r s w e).
+Next Obligation. Admitted.
+Next Obligation. Admitted.
+
+Program Instance RWSE_Applicative {r s w e : Type} :
+  ApplicativeLaws (@RWSE r s w e).
+Next Obligation. Admitted.
+Next Obligation. Admitted.
+Next Obligation. Admitted.
+
+Program Instance RWSE_Monad {r s w e : Type} :
+  MonadLaws (@RWSE r s w e).
+Next Obligation. Admitted.
+Next Obligation. Admitted.
+Next Obligation. Admitted.
+
+End RWSELaws.
