src/ilist.v
@@ -31,4 +31,22 @@ Equations isplit `(xs : ilist (l ++ l')) : ilist l * ilist l'  :=
     | (xs', ys) => ((x, xs'), ys)
   }.
 
+Equations ilist_ind (P : ∀ (l : list A), ilist l → Prop)
+          (Pinil : P [] tt)
+          (Picons : ∀ (a : A) (b : B a) (l : list A) (il : ilist l),
+              P l il → P (a :: l) (b, il))
+          (l : list A) (il : ilist l) : P l il :=
+  ilist_ind P Pinil Picons [] tt := Pinil;
+  ilist_ind P Pinil Picons (a :: l) (b, il) :=
+    Picons a b l il (ilist_ind P Pinil Picons l il).
+
+Equations ilist_rect (P : ∀ (l : list A), ilist l → Type)
+          (Pinil : P [] tt)
+          (Picons : ∀ (a : A) (b : B a) (l : list A) (il : ilist l),
+              P l il → P (a :: l) (b, il))
+          (l : list A) (il : ilist l) : P l il :=
+  ilist_rect P Pinil Picons [] tt := Pinil;
+  ilist_rect P Pinil Picons (a :: l) (b, il) :=
+    Picons a b l il (ilist_rect P Pinil Picons l il).
+
 End ilist.
